proof: have a version of the ERC-20 that compiles without State.Trait

CoqOfRust/M.v
@@ -1,7 +1,7 @@
 (** The definition of a Rust monad. *)
 (** based on experiments.MonadExperiments *)
 
-Module State.
+(* Module State.
   Class Trait (State Address : Set) : Type := {
     get_Set : Address -> Set;
     read (a : Address) : State -> option (get_Set a);
@@ -33,60 +33,101 @@ Module State.
         end;
         }.
   End Valid.
-End State.
+End State. *)
 
-Module MutRef.
-  Inductive t `{State.Trait} : Set -> Set :=
-  | Make (a : Address) : t (State.get_Set a).
-End MutRef.
-Definition MutRef `{State.Trait} := MutRef.t.
+Inductive sigS {A : Type} (P : A -> Set) : Set :=
+| existS : forall (x : A), P x -> sigS P.
+
+Reserved Notation "{ x @ P }" (at level 0, x at level 99).
+Reserved Notation "{ x : A @ P }" (at level 0, x at level 99).
+Reserved Notation "{ ' pat : A @ P }"
+  (at level 0, pat strict pattern, format "{ ' pat : A @ P }").
+
+Notation "{ x @ P }" := (sigS (fun x => P)) : type_scope.
+Notation "{ x : A @ P }" := (sigS (A := A) (fun x => P)) : type_scope.
+Notation "{ ' pat : A @ P }" := (sigS (A := A) (fun pat => P)) : type_scope.
 
 Module Ref.
-  Inductive t `{State.Trait} (A : Set) : Set :=
+  Inductive t (A : Set) : Set :=
   | Immutable : A -> t A
-  | OfMutRef : MutRef A -> t A.
-  Arguments Immutable {_ _ _ _}.
-  Arguments OfMutRef {_ _ _ _}.
+  | MutRef : forall {Address : Set}, Address -> t A.
+  Arguments Immutable {_}.
+  Arguments MutRef {_ _}.
 End Ref.
-Definition Ref `{State.Trait} := Ref.t.
+Definition Ref := Ref.t.
 
-Module RawMonad.
-  Inductive t `{State.Trait} (A : Set) : Set :=
+Module Primitive.
+  Inductive t : Set -> Set :=
+  | StateAlloc {A : Set} : A -> t (Ref.t A)
+  | StateRead {Address A : Set} : Address -> t A
+  | StateWrite {Address A : Set} : Address -> A -> t unit.
+End Primitive.
+Definition Primitive : Set -> Set := Primitive.t.
+
+Module LowM.
+  Inductive t (A : Set) : Set :=
   | Pure : A -> t A
   | Bind {B : Set} : t B -> (B -> t A) -> t A
-  (** [None] when we allocate an immediate value *)
-  | AddressOracle {B : Set} : (option (MutRef B) -> t A) -> t A
-  (** Useful for example to catch the `Return` exception of a function *)
+  | CallPrimitive : Primitive A -> t A
   | Cast {B : Set} : B -> t A
   | Impossible : t A.
-  Arguments Pure {_ _ _ _}.
-  Arguments Bind {_ _ _ _ _}.
-  Arguments AddressOracle {_ _ _ _ _}.
-  Arguments Cast {_ _ _ _ _}.
-  Arguments Impossible {_ _ _ _}.
+  Arguments Pure {_}.
+  Arguments Bind {_ _}.
+  Arguments CallPrimitive {_}.
+  Arguments Cast {_ _}.
+  Arguments Impossible {_}.
 
-  Definition smart_bind `{State.Trait} {A B : Set} (e1 : t A) (e2 : A -> t B) :
-    t B :=
+  Definition smart_bind {A B : Set} (e1 : t A) (e2 : A -> t B) : t B :=
     match e1 with
     | Pure v1 => e2 v1
     | _ => Bind e1 e2
     end.
-End RawMonad.
-Definition RawMonad `{State.Trait} := RawMonad.t.
+End LowM.
+Definition LowM : Set -> Set := LowM.t.
 
-Module Run.
-  Inductive t `{State.Trait} {A : Set} : RawMonad A -> A -> Prop :=
-  | Pure (v : A) : t (RawMonad.Pure v) v
-  | Bind {B : Set} (e1 : RawMonad B) (e2 : B -> RawMonad A) (v1 : B) (v2 : A) :
-    t e1 v1 ->
-    t (e2 v1) v2 ->
-    t (RawMonad.Bind e1 e2) v2
-  | AddressOracle {B : Set}
-      (r : option (MutRef B)) (e : option (MutRef B) -> RawMonad A) (v : A) :
-    t (e r) v ->
-    t (RawMonad.AddressOracle e) v
-  | Cast (v : A) : t (RawMonad.Cast v) v.
-End Run.
+(* Module Run.
+  Inductive t `{State.Trait} :
+      forall {A : Set},
+      LowM A -> State -> A -> State -> Prop :=
+  | Pure {A : Set} (state : State) (v : A) :
+    t (LowM.Pure v) state v state
+  | Bind {A B : Set} (e1 : LowM B) (e2 : B -> LowM A)
+      (state state1 state2 : State)
+      (v1 : B) (v2 : A) :
+    t e1 state v1 state1 ->
+    t (e2 v1) state1 v2 state2 ->
+    t (LowM.Bind e1 e2) state v2 state2
+  | CallPrimitiveStateAllocNone {A : Set} (state : State) (v : A) :
+    t (LowM.CallPrimitive (Primitive.StateAlloc v))
+      state
+      (Ref.Immutable v)
+      state
+  | CallPrimitiveStateAllocSome
+      {address : Address} (v : State.get_Set address)
+      (state state' : State) :
+    State.read address state = None ->
+    State.alloc_write address state v = Some state' ->
+    t (LowM.CallPrimitive (Primitive.StateAlloc v))
+      state
+      (Ref.MutRef (A := State.get_Set address) address)
+      state'
+  | CallPrimitiveStateRead
+      {address : Address} (v : State.get_Set address) (state : State) :
+    State.read address state = Some v ->
+    t (LowM.CallPrimitive (Primitive.StateRead address))
+      state
+      v
+      state
+  | CallPrimitiveStateWrite
+      {address : Address} (v : State.get_Set address) (state state' : State) :
+    State.alloc_write address state v = Some state' ->
+    t (LowM.CallPrimitive (Primitive.StateWrite address v))
+      state
+      tt
+      state'
+  | Cast {A : Set} (state : State) (v : A) :
+    t (LowM.Cast v) state v state.
+End Run. *)
 
 Module Exception.
   Inductive t : Set :=
@@ -100,20 +141,20 @@ Module Exception.
   (** exception for potential non-termination *)
   | NonTermination : t.
 End Exception.
-Definition Exception := Exception.t.
+Definition Exception : Set := Exception.t.
 
-Definition M `{State.Trait} (A : Set) : Set :=
-  nat -> State -> RawMonad ((A + Exception) * State).
+Definition M (A : Set) : Set :=
+  nat -> LowM (A + Exception).
 
-Definition pure `{State.Trait} {A : Set} (v : A) : M A :=
-  fun fuel s => RawMonad.Pure (inl v, s).
+Definition pure {A : Set} (v : A) : M A :=
+  fun fuel => LowM.Pure (inl v).
 
-Definition bind `{State.Trait} {A B : Set} (e1 : M A) (e2 : A -> M B) : M B :=
-  fun fuel s =>
-  RawMonad.smart_bind (e1 fuel s) (fun '(v, s) =>
-  match v with
-  | inl v => e2 v fuel s
-  | inr e => RawMonad.Pure (inr e, s)
+Definition bind {A B : Set} (e1 : M A) (e2 : A -> M B) : M B :=
+  fun fuel =>
+  LowM.smart_bind (e1 fuel) (fun v1 =>
+  match v1 with
+  | inl v1 => e2 v1 fuel
+  | inr error => LowM.Pure (inr error)
   end).
 
 Module Notations.
@@ -127,113 +168,88 @@ Module Notations.
 End Notations.
 Import Notations.
 
-Definition cast `{State.Trait} {A B : Set} (v : A) : M B :=
-  fun _ s => RawMonad.Cast (inl (B := Exception) v, s).
+Definition cast {A B : Set} (v : A) : M B :=
+  fun _fuel => LowM.Cast (inl (B := Exception) v).
 
-Definition raise `{State.Trait} {A : Set} (exception : Exception) : M A :=
-  fun _ s => RawMonad.Pure (inr exception, s).
+Definition raise {A : Set} (exception : Exception) : M A :=
+  fun _fuel => LowM.Pure (inr exception).
 
-Definition return_ `{State.Trait} {A R : Set} (r : R) : M A :=
+Definition return_ {A R : Set} (r : R) : M A :=
   raise (Exception.Return r).
 
-Definition continue `{State.Trait} {A : Set} : M A :=
+Definition continue {A : Set} : M A :=
   raise Exception.Continue.
 
-Definition break `{State.Trait} {A : Set} : M A :=
+Definition break {A : Set} : M A :=
   raise Exception.Break.
 
-Definition panic `{State.Trait} {A B : Set} (v : A) : M B :=
+Definition panic {A B : Set} (v : A) : M B :=
   raise (Exception.Panic v).
 
 (* TODO: define for every (A : Set) in (M A) *)
 (** the definition of a function representing the loop construction *)
-Definition loop `{State.Trait} (m : M unit) : M unit :=
-  fix F (fuel : nat) (s : State) {struct fuel} :=
+Definition loop (m : M unit) : M unit :=
+  fix F (fuel : nat) {struct fuel} :=
     match fuel with
-    | 0 => RawMonad.Pure (inr Exception.NonTermination, s)
+    | 0 => LowM.Pure (inr Exception.NonTermination)
     | S fuel' =>
-      RawMonad.smart_bind (m fuel s) (fun '(v, s) =>
+      LowM.smart_bind (m fuel) (fun v =>
         match v with
         (* only Break ends the loop *)
-        | inl tt                 => F fuel' s
-        | inr Exception.Continue => F fuel' s
-        | inr Exception.Break    => RawMonad.Pure (inl tt, s)
+        | inl tt                 => F fuel'
+        | inr Exception.Continue => F fuel'
+        | inr Exception.Break    => LowM.Pure (inl tt)
         (* every other exception is kept *)
         | inr (Exception.Return _)
         | inr (Exception.Panic _)
-        | inr Exception.NonTermination => RawMonad.Pure (v, s)
+        | inr Exception.NonTermination => LowM.Pure (v)
         end
       )
     end.
 
-Definition alloc `{State.Trait} {A : Set} (v : A) : M (Ref A) :=
-  fun fuel s =>
-  RawMonad.AddressOracle (B := A) (fun r =>
-  match r with
-  | None => RawMonad.Pure (inl (Ref.Immutable v), s)
-  | Some r =>
-    match r, v with
-    | MutRef.Make a, _ =>
-      match State.read a s with
-      | Some _ => RawMonad.Impossible
-      | None =>
-        match State.alloc_write a s v with
-        | Some s => RawMonad.Pure (inl (Ref.OfMutRef (MutRef.Make a)), s)
-        | None => RawMonad.Impossible
-        end
-      end
-    end
-  end).
+Definition alloc {A : Set} (v : A) : M (Ref A) :=
+  fun _fuel =>
+  LowM.smart_bind (LowM.CallPrimitive (Primitive.StateAlloc v)) (fun ref =>
+  LowM.Pure (inl ref)).
 
-Definition read `{State.Trait} {A : Set} (r : Ref A) : M A :=
-  fun fuel s =>
+Definition read {A : Set} (r : Ref A) : M A :=
+  fun _fuel =>
   match r with
-  | Ref.Immutable v => RawMonad.Pure (inl v, s)
-  | Ref.OfMutRef r =>
-    match r with
-    | MutRef.Make a =>
-      match State.read a s with
-      | None => RawMonad.Impossible
-      | Some v => RawMonad.Pure (inl v, s)
-      end
-    end
+  | Ref.Immutable v => LowM.Pure (inl v)
+  | Ref.MutRef address =>
+    LowM.smart_bind (LowM.CallPrimitive (Primitive.StateRead address)) (fun v =>
+    LowM.Pure (inl v))
   end.
 
-Definition write `{State.Trait} {A : Set} (r : Ref A) (v : A) : M unit :=
-  fun fuel s =>
+Definition write {A : Set} (r : Ref A) (v : A) : M unit :=
+  fun _fuel =>
   match r with
-  | Ref.Immutable _ => RawMonad.Impossible
-  | Ref.OfMutRef r =>
-    match r, v with
-    | MutRef.Make a, _ =>
-      match State.alloc_write a s v with
-      | None => RawMonad.Impossible
-      | Some s => RawMonad.Pure (inl tt, s)
-      end
-    end
+  | Ref.Immutable _ => LowM.Impossible
+  | Ref.MutRef address =>
+    LowM.smart_bind
+      (LowM.CallPrimitive (Primitive.StateWrite address v))
+      (fun _ => LowM.Pure (inl tt))
   end.
 
-Definition impossible `{State.Trait} {A : Set} : M A :=
-  fun _ _ => RawMonad.Impossible.
+Definition impossible {A : Set} : M A :=
+  fun _fuel => LowM.Impossible.
 
 (** Used for the definitions of "const". *)
 (* @TODO: Give a definition for [run]. There should be an additional parameter
    witnessing that the calculation is possible. *)
-Parameter run : forall `{State.Trait} {A : Set}, M A -> A.
+Parameter run : forall {A : Set}, M A -> A.
 
-Definition Val `{State.Trait} (A : Set) : Set := Ref A.
+Definition Val (A : Set) : Set := Ref A.
 
-Definition catch `{State.Trait} {A : Set}
-    (body : M A) (handler : Exception -> M A) :
-    M A :=
-  fun fuel state =>
-  RawMonad.smart_bind (body fuel state) (fun '(result, state) =>
+Definition catch {A : Set} (body : M A) (handler : Exception -> M A) : M A :=
+  fun fuel =>
+  LowM.smart_bind (body fuel) (fun result =>
   match result with
-  | inl v => RawMonad.Pure (inl v, state)
-  | inr exception => handler exception fuel state
+  | inl v => LowM.Pure (inl v)
+  | inr exception => handler exception fuel
   end).
 
-Definition function_body `{State.Trait} {A : Set} (body : M A) : M A :=
+Definition function_body {A : Set} (body : M A) : M A :=
   catch body (fun exception =>
   match exception with
   | Exception.Return r => cast r
