CoqOfRust/_std/io.v
@@ -38,10 +38,10 @@ Require CoqOfRust.core.result_types.
 Module Error.
   Parameter t : Set.
 End Error.
-Definition Error `{State.Trait} : Set :=
+Definition Error : Set :=
   M.Val Error.t.
 
-Definition Result `{State.Trait} (T : Set) : Set :=
+Definition Result (T : Set) : Set :=
   core.result_types.Result T Error.t.
 
 (* pub struct BorrowedBuf<'data> { /* private fields */ } *)
@@ -85,7 +85,7 @@ pub trait Write {
 }
 *)
 Module Write.
-  Class Trait `{State.Trait} (Self : Set) : Set := { 
+  Class Trait (Self : Set) : Set := { 
     write : mut_ref Self -> ref (slice u8) -> Result usize;
     flush : mut_ref Self -> Result unit;
     write_vectored : mut_ref Self -> ref (slice IoSlice) -> Result usize;
@@ -327,13 +327,13 @@ pub enum SeekFrom {
 }
 *)
 Module SeekFrom.
-  Inductive t `{State.Trait} : Set :=
+  Inductive t : Set :=
   | Start : u64 -> t
   | End : i64 -> t
   | Current : i64 -> t
   .
 End SeekFrom.
-Definition SeekFrom `{State.Trait} := SeekFrom.t.
+Definition SeekFrom := SeekFrom.t.
 
 (* ********TRAITS******** *)
 (* 
@@ -351,7 +351,7 @@ pub trait IsTerminal: Sealed {
 }
 *)
 Module IsTerminal.
-  Class Trait `{State.Trait} (Self : Set) : Set := { 
+  Class Trait (Self : Set) : Set := { 
     is_terminal : ref Self -> bool;
   }.
 End IsTerminal.
@@ -380,7 +380,7 @@ pub trait Read {
 }
 *)
 Module Read.
-  Class Trait `{State.Trait} (Self : Set) : Set := { 
+  Class Trait (Self : Set) : Set := { 
     read : mut_ref Self -> mut_ref (slice u8) -> Result usize;
     read_vectored : mut_ref Self -> mut_ref (slice IoSliceMut) -> Result usize;
     is_read_vectored : ref Self -> bool;
@@ -413,7 +413,7 @@ pub trait BufRead: Read {
 }
 *)
 Module BufRead.
-  Class Trait `{State.Trait} (Self : Set) `{Read.Trait Self}: Set := { 
+  Class Trait (Self : Set) `{Read.Trait Self}: Set := { 
     fill_buf : mut_ref Self -> Result (ref (slice u8));
     consume : mut_ref Self -> usize -> unit;
     has_data_left : mut_ref Self -> Result bool;
@@ -437,7 +437,7 @@ pub trait Seek {
 }
 *)
 Module Seek.
-  Class Trait `{State.Trait} (Self : Set) : Set := { 
+  Class Trait (Self : Set) : Set := { 
     seek : mut_ref Self -> SeekFrom -> Result u64;
     rewind : mut_ref Self -> Result unit;
     stream_len : mut_ref Self -> Result u64;
@@ -464,5 +464,5 @@ End Seek.
 *)
 
 Module stdio.
-  Parameter _print : forall `{State.Trait}, fmt.Arguments -> M unit.
+  Parameter _print : fmt.Arguments -> M unit.
 End stdio.
