CoqOfRust/core/convert.v
@@ -40,14 +40,12 @@ where
 }
 *)
 Module AsMut.
-  Class Trait `{State.Trait} (Self : Set) {T : Set} : Set := {
+  Class Trait (Self : Set) {T : Set} : Set := {
     as_mut : mut_ref Self -> M (mut_ref T);
   }.
 End AsMut.
 
-Module AsMut_instances. Section AsMut_instances.
-  Context `{State.Trait}.
-
+Module AsMut_instances.
   Global Instance I_str : AsMut.Trait str (T := str).
   Admitted.
 
@@ -56,7 +54,7 @@ Module AsMut_instances. Section AsMut_instances.
 
   Global Instance I_array {T : Set} : AsMut.Trait (array T) (T := slice T).
   Admitted.
-End AsMut_instances. End AsMut_instances.
+End AsMut_instances.
 
 (* 
 pub trait AsRef<T>
@@ -68,14 +66,12 @@ where
 }
 *)
 Module AsRef.
-  Class Trait `{State.Trait} (Self : Set) {T : Set} : Set := {
+  Class Trait (Self : Set) {T : Set} : Set := {
     as_ref : ref Self -> M (ref T);
   }.
 End AsRef.
 
-Module AsRef_instances. Section AsRef_instances.
-  Context `{State.Trait}.
-
+Module AsRef_instances.
   Global Instance I_str : AsRef.Trait str (T := str).
   Admitted.
 
@@ -84,7 +80,7 @@ Module AsRef_instances. Section AsRef_instances.
 
   Global Instance I_array {T : Set} : AsRef.Trait (array T) (T := slice T).
   Admitted.
-End AsRef_instances. End AsRef_instances.
+End AsRef_instances.
 
 (* 
 pub trait From<T>: Sized {
@@ -93,7 +89,7 @@ pub trait From<T>: Sized {
 }
 *)
 Module From.
-  Class Trait (Self : Set) {T : Set} `{State.Trait} : Set := {
+  Class Trait (Self : Set) {T : Set} : Set := {
     from : T -> M Self;
   }.
 End From.
@@ -105,7 +101,7 @@ pub trait Into<T>: Sized {
 }
 *)
 Module Into.
-  Class Trait (Self : Set) {T : Set } `{State.Trait} : Set := {
+  Class Trait (Self : Set) {T : Set } : Set := {
     into : Self -> M T;
   }.
 End Into.
@@ -113,7 +109,6 @@ End Into.
 Module Impl_Into_for_T.
   Section Impl_Into_for_T.
     Context {T U : Set}.
-    Context `{State.Trait}.
     Context `{From.Trait U (T := T)}.
 
     Definition Self := T.
@@ -139,13 +134,13 @@ pub trait TryFrom<T>: Sized {
 }
 *)
 Module TryFrom.
-  Class Trait (Self : Set) {T : Set} `{State.Trait} : Type := {
+  Class Trait (Self : Set) {T : Set} : Type := {
     Error : Set;
 
     try_from : T -> M (Result Self Error);
   }.
 
-  Global Instance AssociatedFunction_try_from `{State.Trait}
+  Global Instance AssociatedFunction_try_from
       (Self T : Set) {_ : Trait Self (T := T)} :
     Notation.DoubleColon Self "try_from" := {
     Notation.double_colon := try_from;
@@ -161,15 +156,14 @@ pub trait TryInto<T>: Sized {
 }
 *)
 Module TryInto.
-  Class Trait (Self : Set) {T : Set} `{State.Trait} : Type := { 
+  Class Trait (Self : Set) {T : Set} : Type := { 
     Error : Set;
     try_into : Self -> M (Result T Error);
   }.
 
-  Global Instance Method_try_into (Self T : Set) `{State.Trait}
-      {_ : Trait Self (T := T)} :
+  Global Instance Method_try_into (Self T : Set) {_ : Trait Self (T := T)} :
     Notation.Dot "try_into" := {
-    Notation.dot `{State.Trait} := try_into;
+    Notation.dot := try_into;
   }.
 End TryInto.
 
@@ -188,7 +182,6 @@ where
 *)
 Module Impl_TryInto_for_T.
   Section Impl_TryInto_for_T.
-    Context `{State.Trait}.
     Context {T U : Set}.
     Context {H_TryFrom : TryFrom.Trait U (T := T)}.
 
