CoqOfRust/core/marker.v
@@ -92,7 +92,7 @@ End Unsize.
 (* pub trait Copy: Clone { } *)
 Module Copy.
   Unset Primitive Projections.
-  Class Trait `{State.Trait} (Self : Set) : Set := {
+  Class Trait (Self : Set) : Set := {
     _ :: core.clone.Clone.Trait Self;
   }.
   Set Primitive Projections.
