CoqOfRust/_std/collections.v
@@ -321,15 +321,15 @@ Module map.
   (* pub struct DefaultHasher(_); *)
   Module DefaultHasher.
     Parameter t : Set.
-    Definition new `{State.Trait} (_ : unit) : M t. Admitted.
+    Definition new (_ : unit) : M t. Admitted.
 
-    Global Instance DefaultHasher_new `{State.Trait} :
+    Global Instance DefaultHasher_new :
       Notation.DoubleColon t "new" := {
       Notation.double_colon := new
     }.
   End DefaultHasher.
 
-  Definition DefaultHasher := DefaultHasher.t.  
+  Definition DefaultHasher := DefaultHasher.t.
   (* pub struct Drain<'a, K: 'a, V: 'a> { /* private fields */ } *)
   Module Drain.
     Parameter t : Set -> Set -> Set.
