CoqOfRust/alloc/fmt.v
@@ -3,6 +3,4 @@ Require Import CoqOfRust.lib.lib.
 Require CoqOfRust.alloc.string.
 Require CoqOfRust.core.fmt.
 
-Parameter format :
-  forall `{H : State.Trait},
-  core.fmt.Arguments -> M (H := H) alloc.string.String.
+Parameter format : core.fmt.Arguments -> M alloc.string.String.
